## Efficiency definitions

Total-to-total esficiency definition
$$
\eta_{\text{tt}}=\frac{h_{01}-h_{02}}{h_{01}-h_{02s}}=\frac{h_{01}-h_{02}}{h_{01}-h_{2s}-{v_2^2}/{2}}
$$

Total-to-static esficiency definition
$$
\eta_{\text{ts}}=\frac{h_{01}-h_{02}}{h_{01}-h_{0s}}
$$

Taking the inverse of $\eta_{\text{tt}}$ we see that:
$$
\frac{1}{\eta_{\text{tt}}}=\frac{h_{01}-h_{2s}-{v_2^2}/{2}}{h_{01}-h_{02}}=\frac{1}{\eta_{\text{ts}}}-\frac{v_2^2 / 2}{h_{01}-h_{02}} = \frac{1}{\eta_{\text{ts}}} - \Delta \eta_{ke}
$$

Solving for the total-to-total efficiency we get:

$$
\eta_{\text{tt}}=\frac{\eta_{\text{ts}}}{(1-  \eta_{\text{ts}} \,\Delta \eta_{ke})} 
$$


Alternatively, solving for the total-to-static efficiency we get

$$
\eta_{\text{ts}}=\frac{\eta_{\text{tt}}}{(1 + \eta_{\text{tt}} \,\Delta \eta_{ke})} 
$$

From these formulas it is clear that $\eta_{\text{tt}} > \eta_{\text{ts}}$ for $\Delta \eta_{ke}>0$.

